Polynomials.Multiplication.fst
@@ -30,7 +30,18 @@ let monomial #c (r: commutative_ring #c) (a:c) (degree: nat)
   equals_self r a;
   if degree=0 then create 1 a
   else (stream_of_zeros #c #r (degree)) $+ a 
- 
+
+let nth_of_monomial #c (r: commutative_ring #c) (a:c) (deg: nat)
+  : Lemma (forall (i: nat). (nth (monomial r a deg) i == (if (i=deg) then a else r.addition.neutral))) = ()
+
+let monomial_length_is_deg #c (r: commutative_ring #c) (a:c) (deg: nat) : Lemma (length (monomial r a deg) = (1+deg)) = ()
+
+let monomial_leading_coefficient_is_a #c (r: commutative_ring #c) (a:c) (deg: nat)
+  : Lemma (nth (monomial r a deg) deg == a) = ()
+  
+let monomial_other_coefficients_are_zeros #c (r: commutative_ring #c) (a:c) (deg: nat) (i: nat{i<>deg})
+  : Lemma (nth (monomial r a i) deg == r.addition.neutral) = ()
+
 let monomials_equality_lemma #c (r: commutative_ring #c) (a:c) (b:c{r.eq a b}) (degree: nat)
   : Lemma (ensures ncpoly_eq (monomial r a degree) (monomial r b degree)) (decreases degree) 
   = if degree > 0 then eq_of_snoc (stream_of_zeros #c #r degree) a b  
@@ -194,15 +205,452 @@ let rec poly_sum_batch #c (#r: commutative_ring #c) (p: seq (noncompact_poly_ove
          (ensures fun s -> forall (x:index_for s). index s x == noncompact_poly_add (index p x) (index q x))
          (decreases length p) =         
     if length p = 0 then empty
-    else Seq.Properties.cons (noncompact_poly_add (Seq.Properties.head p) (Seq.Properties.head q)) (poly_sum_batch (Seq.Properties.tail p) (Seq.Properties.tail q))
+    else Seq.Properties.cons (noncompact_poly_add (Seq.Properties.head p) (Seq.Properties.head q)) 
+                             (poly_sum_batch (Seq.Properties.tail p) (Seq.Properties.tail q))
           
+ 
+let rec big_sum #c #eq (cm: Algebra.CommMonoid.Equiv.cm c eq) 
+                 (n0: int) (nk: int{nk >= n0}) (expr: (t:int{t>=n0 /\ t<=nk}) -> c) 
+                 : Pure (c) 
+                 (requires True)  
+                 (ensures (fun (x:c) -> ( (nk=n0) ==> (x == expr nk )))) 
+                 (decreases nk-n0) = 
+  if nk = n0 then expr nk
+  else (big_sum cm n0 (nk-1) expr) `cm.mult` expr nk
 
-let fold_of_sum #c (#r: commutative_ring #c) (p: seq (noncompact_poly_over_ring r)) (q: (seq (noncompact_poly_over_ring r)){length q = length p})
-  : Lemma (FStar.Seq.Permutation.foldm_snoc (poly_add_commutative_monoid r) (poly_sum_batch p q) 
-          `noncompact_poly_eq` 
-          noncompact_poly_add (Seq.Permutation.foldm_snoc (poly_add_commutative_monoid r) p)
-                              (Seq.Permutation.foldm_snoc (poly_add_commutative_monoid r) q)) = admit()
+let rec big_sum_equality #c #eq (cm: Algebra.CommMonoid.Equiv.cm c eq) (n0: int) (nk: int{nk>=n0}) (expr1: int->c) (expr2: int->c)
+  : Lemma (requires (forall (i: int{i>=n0 && i<=nk}). expr1 i == expr2 i))
+          (ensures big_sum cm n0 nk expr1 == big_sum cm n0 nk expr2)
+          (decreases nk-n0) = 
+  if nk>n0 then big_sum_equality cm n0 (nk-1) expr1 expr2 
+  
 
+let big_sum_snoc #c #eq (cm: Algebra.CommMonoid.Equiv.cm c eq) 
+                 (n0: nat) (nk: nat{nk > n0}) (expr: (t:nat{t>=n0 /\ t<=nk}) -> c) 
+                 : Lemma (big_sum cm n0 nk expr == big_sum cm n0 (nk-1) expr `cm.mult` (expr nk)) = ()
+
+unfold let foldm_snoc #c #eq = FStar.Seq.Permutation.foldm_snoc #c #eq
+
+#push-options "--ifuel 0 --fuel 1 --z3rlimit 3 --query_stats"
+let rec big_sum_equals_foldm #c #eq 
+                             (cm: Algebra.CommMonoid.Equiv.cm c eq) 
+                             (n0:int) 
+                             (nk:int{nk>=n0}) 
+                             (expr: (t:int{t>=n0 && t<=nk})->c)
+  : Lemma (ensures big_sum cm n0 nk expr `eq.eq` foldm_snoc cm (init (nk+1-n0) (fun (i: under (nk+1-n0)) -> expr (n0+i))))
+          (decreases nk-n0) = 
+  if (nk=n0) then (
+   let ts = init (nk+1-n0) (fun (i: under (nk+1-n0)) -> expr (n0+i)) in
+   lemma_eq_elim (create 1 (expr nk)) ts; 
+   Seq.Permutation.foldm_snoc_singleton cm (expr nk);   
+   eq.symmetry (foldm_snoc cm ts) (expr nk);
+   eq.reflexivity (expr nk); 
+   eq.transitivity (big_sum cm n0 nk expr) (expr nk) (foldm_snoc cm ts); 
+   ()
+  )
+  else (
+    let lhs = big_sum cm n0 nk expr in
+    let rhs = foldm_snoc cm (init (nk+1-n0) (fun (i: under (nk+1-n0)) -> expr (n0+i))) in
+    let fullseq = init (nk+1-n0) (fun (i: under (nk+1-n0)) -> expr (n0+i)) in    
+    let subseq = init (nk-n0) (fun (i: under (nk-n0)) -> expr (n0+i)) in
+    let subsum = big_sum cm n0 (nk-1) expr in
+    let fullfold = foldm_snoc cm fullseq in
+    let subfold = foldm_snoc cm subseq in
+    let last = expr nk in
+    let op = cm.mult in
+    big_sum_equals_foldm cm n0 (nk-1) expr;    
+    lemma_eq_elim (init ((nk-1)+1-n0) (fun (i: under ((nk-1)+1-n0)) -> expr (n0+i))) subseq;
+    // yes! [(nk-1)+1-n0 == nk-n0] is not enough!
+    // assert (subsum `eq.eq` foldm_snoc cm subseq); -- comes from recursion
+    // assert (lhs == subsum `cm.mult` (expr nk)); -- by the definition of big_sum
+    lemma_eq_elim (fst (un_snoc fullseq)) subseq; // subseq is literally (liat fullseq)
+    // what we already have: rhs == (expr nk) + (foldm_snoc cm subseq)
+    // what we want: rhs `eq.eq` (foldm_snoc cm subseq) + (expr nk)
+    cm.commutativity last subfold;
+    eq.reflexivity last; 
+    // subsum * last `eq` subfold * last -- from congruence
+    cm.congruence subsum last subfold last;
+    eq.symmetry rhs (subfold `op` last);
+    eq.transitivity lhs (subfold `op` last) rhs;
+    ()
+  )
+
+let bounds_lemma (n0:int) (nk: int{nk>=n0}) (i:nat{i<(nk+1-n0)}) : Lemma (n0+i >= n0 /\ n0+i <= nk) = ()
+
+let fold_decomposition_aux #c #eq (cm: Algebra.CommMonoid.Equiv.cm c eq)
+                           (n0: int) 
+                           (nk: int{nk=n0}) 
+                           (expr1 expr2: (t:int{t>=n0 /\ t<=nk}) -> c)
+  : Lemma (foldm_snoc cm (init (nk+1-n0) (fun i -> expr1 (n0+i) `cm.mult` expr2 (n0+i))) `eq.eq`
+           cm.mult (foldm_snoc cm (init (nk+1-n0) (fun i -> expr1 (n0+i)))) 
+                   (foldm_snoc cm (init (nk+1-n0) (fun i -> expr2 (n0+i))))) =  
+    lemma_eq_elim (init (nk+1-n0) (fun i -> expr1 (n0+i) `cm.mult` expr2 (n0+i))) 
+                  (create 1 (expr1 n0 `cm.mult` expr2 n0));
+    Seq.Permutation.foldm_snoc_singleton cm (expr1 n0 `cm.mult` expr2 n0);
+    let ts = (init (nk+1-n0) (fun i -> expr1 (n0+i) `cm.mult` expr2 (n0+i))) in
+    let lhs = foldm_snoc cm ts in
+    let ts1 = (init (nk+1-n0) (fun i -> expr1 (n0+i))) in
+    let ts2 = (init (nk+1-n0) (fun i -> expr2 (n0+i))) in
+    let rhs = cm.mult (foldm_snoc cm ts1) (foldm_snoc cm ts2) in
+    eq.symmetry (foldm_snoc cm ts) (expr1 n0 `cm.mult` expr2 n0);
+    eq.reflexivity ((fun (i:nat{i<(nk+1-n0)}) -> bounds_lemma n0 nk i;  expr1 (n0+i) `cm.mult` expr2 (n0+i)) (nk-n0)); 
+    assert (foldm_snoc cm ts `eq.eq`  ((fun i -> bounds_lemma n0 nk i; 
+                                              expr1 (n0+i) `cm.mult` expr2 (n0+i)) 
+                                      (nk-n0))); //lambda call.
+    assert ( ((fun i -> bounds_lemma n0 nk i; expr1 (n0+i) `cm.mult` expr2 (n0+i)) (nk-n0)) ==
+      cm.mult (expr1 (n0)) (expr2 (n0)));
+    assert (lhs `eq.eq` cm.mult (expr1 nk) (expr2 nk));  
+    assert (equal ts1 (create 1 (expr1 nk)));
+    Seq.Permutation.foldm_snoc_singleton cm (expr1 nk);    
+    assert (eq.eq (foldm_snoc cm ts1) (expr1 nk));
+    Seq.Permutation.foldm_snoc_singleton cm (expr2 nk);    
+    assert (eq.eq (foldm_snoc cm ts2) (expr2 nk));
+    cm.congruence (foldm_snoc cm ts1) (foldm_snoc cm ts2) (expr1 nk) (expr2 nk);
+    assert (rhs `eq.eq` (cm.mult (expr1 nk) (expr2 nk)));
+    eq.symmetry rhs (cm.mult (expr1 nk) (expr2 nk));
+    eq.transitivity lhs (cm.mult (expr1 nk) (expr2 nk)) rhs 
+
+let aux_shuffle_lemma #c #eq (cm: Algebra.CommMonoid.Equiv.cm c eq) (s1 s2 l1 l2: c)
+  : Lemma (((s1 `cm.mult` s2) `cm.mult` (l1 `cm.mult` l2)) `eq.eq`  
+           ((s1 `cm.mult` l1) `cm.mult` (s2 `cm.mult` l2))) =  
+  Classical.forall_intro eq.reflexivity;
+  Classical.forall_intro_2 (Classical.move_requires_2 eq.symmetry);
+  Classical.forall_intro_2 (Classical.move_requires_2 cm.commutativity);
+  Classical.forall_intro_3 (Classical.move_requires_3 eq.transitivity); 
+  let (+) = cm.mult in
+  let (=) = eq.eq in
+  let assoc = cm.associativity in
+  let s12 = s1 + s2 in
+  let lhs = (s1+s2)+(l1+l2) in
+  assoc s12 l1 l2 ;
+  assert (lhs = (s12 + l1) + l2);
+  assoc s1 s2 l1;
+  assert (((s1+s2)+l1) = (s1+(s2+l1)));
+  cm.congruence (s1+s2) l1 (s2+s1) l1;
+  assert (((s1+s2)+l1) = ((s2+s1)+l1));
+  cm.congruence ((s1+s2)+l1) l2 ((s2+s1)+l1) l2;
+  assert (lhs = (((s2+s1)+l1)+l2));
+  assoc s2 s1 l1;
+  cm.congruence ((s2+s1)+l1) l2 (s2+(s1+l1)) l2;
+  assert (lhs = ((s2+(s1+l1))+l2));
+  cm.congruence (s2+(s1+l1)) l2 ((s1+l1)+s2) l2;
+  
+  assert (lhs = (((s1+l1)+s2)+l2));
+  assoc (s1+l1) s2 l2;
+  assert (lhs = ((s1+l1)+(s2+l2)));  
+  ()
+
+#push-options "--ifuel 0 --fuel 1 --z3rlimit 5 --query_stats"
+ 
+#push-options "--ifuel 0 --fuel 1 --z3rlimit 2 --z3refresh --query_stats"
+let rec fold_decomposition_clean #c #eq (cm: Algebra.CommMonoid.Equiv.cm c eq)
+                           (n0: int) 
+                           (nk: int{nk>=n0}) 
+                           (expr1 expr2: int -> c)
+  : Lemma (ensures foldm_snoc cm (init (nk+1-n0) (fun i -> expr1 (n0+i) `cm.mult` expr2 (n0+i)))
+          `eq.eq` (foldm_snoc cm (init (nk+1-n0) (fun i -> expr1 (n0+i))) 
+         `cm.mult` foldm_snoc cm (init (nk+1-n0) (fun i -> expr2 (n0+i)))))
+          (decreases nk-n0) = 
+  if (nk=n0) then fold_decomposition_aux cm n0 nk expr1 expr2  else (  
+    Classical.forall_intro_2 (Classical.move_requires_2 cm.commutativity);
+    Classical.forall_intro_3 (Classical.move_requires_3 eq.transitivity); 
+    let op = cm.mult in
+    let fold s = foldm_snoc #c #eq cm s in
+    let left_func : (i:nat{i<(nk+1-n0)}) -> c = fun i -> expr1 (n0+i) `op` expr2 (n0+i) in
+    let fullseq = init (nk+1-n0) left_func in
+    let lhs = fold fullseq in
+    let right_func1 : (i:nat{i<(nk+1-n0)}) -> c = fun i -> expr1 (n0+i) in
+    let right_func2 : (i:nat{i<(nk+1-n0)}) -> c = fun i -> expr2 (n0+i) in
+    let fullseq_r1 = init (nk+1-n0) right_func1 in
+    let fullseq_r2 = init (nk+1-n0) right_func2 in
+    let rhs = (fold fullseq_r1) `op` (fold fullseq_r2) in
+    fold_decomposition_clean cm n0 (nk-1) expr1 expr2;
+    let subseq = init (nk-n0) left_func in
+    let subfold = fold subseq in
+    let last = left_func (nk-n0) in
+    lemma_eq_elim (fst (un_snoc fullseq)) subseq;    
+    let subseq_r1 = init (nk-n0) right_func1 in
+    let subseq_r2 = init (nk-n0) right_func2 in  
+    lemma_eq_elim subseq (init ((nk-1)+1-n0) (fun i -> expr1 (n0+i) `op` expr2 (n0+i)));       
+    let subfold_r1 = foldm_snoc cm subseq_r1 in
+    let subfold_r2 = foldm_snoc cm subseq_r2 in 
+    lemma_eq_elim subseq_r1 (init ((nk-1)+1-n0) (fun i -> expr1 (n0+i)));
+    lemma_eq_elim subseq_r2 (init ((nk-1)+1-n0) (fun i -> expr2 (n0+i))); 
+    cm.congruence (foldm_snoc cm (init ((nk-1)+1-n0) (fun i -> expr1 (n0+i)))) 
+                  (foldm_snoc cm (init ((nk-1)+1-n0) (fun i -> expr2 (n0+i))))
+                  subfold_r1 subfold_r2; 
+    let last_r1 = right_func1 (nk-n0) in
+    let last_r2 = right_func2 (nk-n0) in
+    lemma_eq_elim (fst (un_snoc fullseq_r1)) subseq_r1; // subseq is literally (liat fullseq)
+    lemma_eq_elim (fst (un_snoc fullseq_r2)) subseq_r2;
+    cm.congruence subfold last (subfold_r1 `op` subfold_r2) last;
+    aux_shuffle_lemma cm subfold_r1 subfold_r2 last_r1 last_r2;    
+    cm.congruence (subfold_r1 `op` last_r1) (subfold_r2 `op` last_r2) (foldm_snoc cm fullseq_r1) (foldm_snoc cm fullseq_r2) 
+) 
+
+type comm_monoid c eq = Algebra.CommMonoid.Equiv.cm c eq 
+
+#push-options "--ifuel 0 --fuel 0 --z3rlimit 1 --query_stats"
+let big_sum_decomposition #c #eq 
+                              (cm: Algebra.CommMonoid.Equiv.cm c eq) 
+                              (n0: int) 
+                              (nk: int{nk>=n0}) 
+                              (expr1 expr2: (t:int{t>=n0 && t<=nk}) -> c)
+  : Lemma (big_sum cm n0 nk (fun (i:int{i>=n0 && i<=nk}) -> expr1 i `cm.mult` expr2 i) 
+   `eq.eq` (cm.mult (big_sum cm n0 nk expr1) (big_sum cm n0 nk expr2))) =  
+    Classical.forall_intro_2 (Classical.move_requires_2 eq.symmetry);
+    Classical.forall_intro_3 (Classical.move_requires_3 eq.transitivity);
+    let op = cm.mult in
+    let make_seq (expr: (t:int{t>=n0 /\ t<=nk}) -> c) = init (nk+1-n0) (fun (i:under (nk+1-n0)) -> expr (n0+i)) in 
+    let sum_expr : ((t:int{t>=n0 /\ t<=nk}) -> c) = fun (i:int{i>=n0 && i<=nk}) -> expr1 i `op` expr2 i in
+    big_sum_equals_foldm cm n0 nk sum_expr; 
+    fold_decomposition_clean cm n0 nk expr1 expr2; 
+    big_sum_equals_foldm cm n0 nk expr1;
+    big_sum_equals_foldm cm n0 nk expr2;
+    cm.congruence (foldm_snoc cm (make_seq expr1)) (foldm_snoc cm (make_seq expr2))
+                  (big_sum cm n0 nk expr1) (big_sum cm n0 nk expr2) 
+
+
+let matrix_seq #c #eq (cm: comm_monoid c eq) (m n: pos) (generator: (under m) -> (under n) -> c)
+  : Pure (z:seq c{length z = m `op_Multiply` n}) 
+         (requires True)
+         (ensures fun x -> ( (forall (i: under m) (j: under n). index x (get_ij m n i j) == generator i j) /\ 
+                           (forall (ij: under (m `op_Multiply` n)). (index x ij) == ( generator (get_i m n ij) (get_j m n ij)))))  = 
+  let ( *) = op_Multiply in                           
+  let mn = m * n in
+  let generator_ij ij = generator (get_i m n ij) (get_j m n ij) in
+  let flat_indices : seq (t:nat{t<mn}) = get_int_range (mn) in 
+  map_seq_len generator_ij flat_indices;
+  let result = map_seq generator_ij flat_indices in
+  let aux (i: under m) (j: under n) 
+    : Lemma (index (map_seq generator_ij flat_indices) (get_ij m n i j) == generator i j) 
+    = 
+      consistency_of_i_j m n i j;
+      consistency_of_ij m n (get_ij m n i j);
+      assert (generator_ij (get_ij m n i j) == generator i j);
+      map_seq_index generator_ij flat_indices (get_ij m n i j);    
+    () in
+  let aux1 (ij: under mn) : Lemma (index (map_seq generator_ij flat_indices) ij == generator_ij ij) 
+    = map_seq_index generator_ij flat_indices ij;
+    () in 
+  Classical.forall_intro aux1;
+  Classical.forall_intro_2 aux;
+  result
+
+#push-options "--ifuel 1 --fuel 0 --z3rlimit 10 --query_stats"
+
+let matrix_snoc #c #eq (cm: comm_monoid c eq) (m n: pos) (generator: (under m) -> (under n) -> c)
+  : Lemma (matrix_seq cm m n generator `equal` append (slice (matrix_seq cm m n generator) 0 ((m-1)*n))
+                                                      (slice (matrix_seq cm m n generator) ((m-1)*n) (m*n))) = ()
+
+let matrix_sum_snoc #c #eq (cm: comm_monoid c eq) (m n: pos) (generator: (under m) -> (under n) -> c)
+  : Lemma (foldm_snoc cm (matrix_seq cm m n generator) `eq.eq` (cm.mult
+           (foldm_snoc cm (slice (matrix_seq cm m n generator) 0 ((m-1)*n)))
+           (foldm_snoc cm (slice (matrix_seq cm m n generator) ((m-1)*n) (m*n))))) = 
+           Seq.Permutation.foldm_snoc_append cm (slice (matrix_seq cm m n generator) 0 ((m-1)*n))
+                                                (slice (matrix_seq cm m n generator) ((m-1)*n) (m*n));
+           lemma_eq_elim (matrix_seq cm m n generator) (append (slice (matrix_seq cm m n generator) 0 ((m-1)*n))
+                                                (slice (matrix_seq cm m n generator) ((m-1)*n) (m*n))) 
+
+let matrix_last_line_equals_big_sum #c #eq (cm: comm_monoid c eq) (m n: pos) (generator: (under m) -> (under n) -> c) 
+  : Lemma (foldm_snoc cm (slice (matrix_seq cm m n generator) ((m-1)*n) (m*n)) `eq.eq` big_sum cm 0 (n-1) (fun (j: under n) -> generator (m-1) j)) = 
+  big_sum_equals_foldm cm 0 (n-1) (fun j -> generator (m-1) j);
+  Classical.forall_intro eq.reflexivity;
+  Classical.forall_intro_2 (Classical.move_requires_2 eq.symmetry);
+  Classical.forall_intro_2 (Classical.move_requires_2 cm.commutativity);
+  Classical.forall_intro_3 (Classical.move_requires_3 eq.transitivity); 
+  
+  assert (big_sum cm 0 (n-1) (fun j -> generator (m-1) j) `eq.eq`  
+          foldm_snoc cm (init ((n-1)+1-0) (fun j -> generator (m-1) (j+0))) 
+          );
+  admit();
+          
+  assert (slice (matrix_seq cm m n generator) ((m-1)*n) (m*n) `equal` init n (fun (j: under n) -> generator (m-1) j));
+  lemma_eq_elim (slice (matrix_seq cm m n generator) ((m-1)*n) (m*n)) (init n (fun (j: under n) -> generator (m-1) j));
+  assert (foldm_snoc cm (slice (matrix_seq cm m n generator) ((m-1)*n) (m*n)) ==
+          foldm_snoc cm (init n (fun (j: under n) -> generator (m-1) j)));
+
+ 
+          ()
+           
+let rec matrix_seq_fold_equals_big_sum #c #eq (cm: comm_monoid c eq) (m n: pos)  (generator: int -> int -> c) 
+  : Lemma (ensures foldm_snoc cm (matrix_seq cm m n generator) `eq.eq` 
+           big_sum cm 0 (m-1) (fun (i:under m) -> big_sum cm 0 (n-1) (fun (j:under n) -> generator i j))) (decreases %[m;n])= 
+  let lhs = foldm_snoc cm (matrix_seq cm m n generator) in
+  let rhs = big_sum cm 0 (m-1) (fun (i:under m) -> big_sum cm 0 (n-1) (fun (j:under n) -> generator i j)) in
+  let matrix = matrix_seq cm m n generator in
+  let line_lemma (i: under m) 
+    : Lemma (big_sum cm 0 (n-1) (fun (j:under n) -> generator i j) `eq.eq` 
+             foldm_snoc cm (slice matrix (i*n) (i*n+n))) = 
+    assert (slice matrix (i*n) (i*n+n) `equal` (init n (fun (j:under n) -> generator i j)));
+    let gen_fun (j: under n) = generator i j in
+    let lhs_bigsum = big_sum cm 0 (n-1) gen_fun in
+    let sliced = slice matrix (i*n) (i*n + n) in
+    lemma_eq_elim (init ((n-1) + 1 - 0) gen_fun) (init n gen_fun);
+    big_sum_equals_foldm cm 0 (n-1) gen_fun;
+    assert (eq.eq (big_sum cm 0 (n-1) gen_fun) (foldm_snoc cm (init n (fun j -> gen_fun (0+j) )  )));
+    admit();
+    lemma_eq_elim sliced (init n (fun (j:under n) -> generator i j));
+    Classical.forall_intro eq.reflexivity;     
+    assert (foldm_snoc cm sliced == foldm_snoc cm (init n (fun (j:under n) -> generator i j)));
+    eq.transitivity (big_sum cm 0 (n-1) gen_fun)
+                    (foldm_snoc cm (init n (fun (j:under n) -> generator i j)))
+                    (foldm_snoc cm sliced);
+    assert (eq.eq (big_sum cm 0 (n-1) gen_fun) (foldm_snoc cm sliced)); 
+    () in
+  if (m=1) then (
+    assert (matrix `equal` slice matrix 0 n);
+    line_lemma 0;
+    assert (foldm_snoc cm (matrix_seq cm m n generator) == foldm_snoc cm (slice matrix 0 n));
+    assert (m-1 = 0); 
+    let general_func i = big_sum cm 0 (m-1) (fun j -> generator i j) in
+      
+    assert (big_sum cm 0 (m-1) general_func == big_sum cm 0 (m-1) (fun j -> generator 0 j));
+    big_sum_equality cm 0 (m-1) general_func (fun j -> generator 0 j);
+    admit();
+    assert (rhs == big_sum cm 0 (m-1) general_func);
+//    assert (rhs == big_sum cm 0 (m-1) outer_func); 
+    ()
+  ) else ( 
+    admit();
+    ()
+  )
+
+
+let double_sum_flatten #c #eq (cm: comm_monoid c eq)
+                              (m0: int) (mk: int{mk>=m0})
+                              (n0: int) (nk: int{nk>=n0})
+                              (expr: int -> int -> c)
+  : Lemma (ensures big_sum cm m0 mk (fun m -> big_sum cm n0 nk (fun n -> expr m n)) `eq.eq`
+                   foldm_snoc cm (init ((mk+1-m0) `op_Multiply` (nk+1-n0)) (fun ij -> expr (ij / (nk+1-n0)) (ij % (nk+1-n0))))) 
+          (decreases %[(mk-m0); (nk-n0)]) = 
+  let lhs = big_sum cm m0 mk (fun m -> big_sum cm n0 nk (fun n -> expr m n)) in
+  let p = (mk+1-m0) in
+  let q = (nk+1-n0) in
+  if (mk=m0) then (
+    assert (mk == m0);
+    assert (p=1);
+    assert (lhs == big_sum cm n0 nk (fun n -> expr mk n));
+    admit();
+    ()
+  ) else admit()
+
+let double_fold_swap #c #eq (cm: comm_monoid c eq)
+                            (m0: int) (mk: int{mk>=m0})
+                            (n0: int) (nk: int{nk>=n0})
+                            (expr: int -> int -> c)
+  : Lemma (ensures big_sum cm m0 mk (fun m -> big_sum cm n0 nk (fun n -> expr m n)) `eq.eq`
+                   big_sum cm n0 nk (fun n -> big_sum cm m0 mk (fun m -> expr m n))) = admit()
+
+let rec fold_decomposition #c #eq (cm: Algebra.CommMonoid.Equiv.cm c eq)
+                           (n0: int) 
+                           (nk: int{nk>=n0}) 
+                           (expr1 expr2: (t:int{t>=n0 /\ t<=nk}) -> c)
+  : Lemma (ensures foldm_snoc cm (init (nk+1-n0) (fun (i:nat{i<(nk+1-n0)}) -> expr1 (n0+i) `cm.mult` expr2 (n0+i))) `eq.eq`
+           cm.mult (foldm_snoc cm (init (nk+1-n0) (fun (i:nat{i<(nk+1-n0)}) -> expr1 (n0+i)))) 
+                   (foldm_snoc cm (init (nk+1-n0) (fun (i:nat{i<(nk+1-n0)}) -> expr2 (n0+i)))))
+          (decreases nk-n0) = 
+  if (nk=n0) then fold_decomposition_aux cm n0 nk expr1 expr2  else (  
+    Classical.forall_intro eq.reflexivity;
+    Classical.forall_intro_2 (Classical.move_requires_2 eq.symmetry);
+    Classical.forall_intro_2 (Classical.move_requires_2 cm.commutativity);
+    Classical.forall_intro_3 (Classical.move_requires_3 eq.transitivity); 
+    let op = cm.mult in
+    let fold s = foldm_snoc #c #eq cm s in
+    let left_func : (i:nat{i<(nk+1-n0)}) -> c = fun (i:nat{i<(nk+1-n0)}) -> expr1 (n0+i) `op` expr2 (n0+i) in
+    let fullseq = init (nk+1-n0) left_func in
+    let lhs = fold fullseq in
+    let right_func1 : (i:nat{i<(nk+1-n0)}) -> c = fun (i:nat{i<(nk+1-n0)}) -> expr1 (n0+i) in
+    let right_func2 : (i:nat{i<(nk+1-n0)}) -> c = fun (i:nat{i<(nk+1-n0)}) -> expr2 (n0+i) in
+    let fullseq_r1 = init (nk+1-n0) right_func1 in
+    let fullseq_r2 = init (nk+1-n0) right_func2 in
+    let rhs = (fold fullseq_r1) `op` (fold fullseq_r2) in
+    fold_decomposition cm n0 (nk-1) expr1 expr2;
+    //assert (foldm_snoc cm (init ((nk-1)+1-n0) (fun i -> expr1 (n0+i) `cm.mult` expr2 (n0+i))) `eq.eq`
+    //       cm.mult (foldm_snoc cm (init ((nk-1)+1-n0) (fun i -> expr1 (n0+i)))) 
+    //               (foldm_snoc cm (init ((nk-1)+1-n0) (fun i -> expr2 (n0+i))))); 
+    let subseq = init (nk-n0) left_func in
+    //lemma_eq_elim (init ((nk-1)+1-n0) left_func) subseq;
+    let subfold = foldm_snoc cm subseq in
+    let last = left_func (nk-n0) in
+    lemma_eq_elim (fst (un_snoc fullseq)) subseq; // subseq is literally (liat fullseq) 
+    //cm.commutativity last subfold;
+    //eq.reflexivity (foldm_snoc cm fullseq);  
+    //assert (foldm_snoc cm fullseq == cm.mult last subfold);
+    //assert (foldm_snoc cm fullseq `eq.eq` cm.mult subfold last);
+    //assert (lhs `eq.eq` cm.mult subfold last); 
+    //assert (rhs == foldm_snoc cm fullseq_r1 `cm.mult` foldm_snoc cm fullseq_r2);
+    let subseq_r1 = init (nk-n0) right_func1 in
+    let subseq_r2 = init (nk-n0) right_func2 in
+    lemma_eq_elim (init ((nk-1)+1-n0) right_func1) subseq_r1;
+    lemma_eq_elim (init ((nk-1)+1-n0) right_func2) subseq_r2; 
+    lemma_eq_elim subseq (init ((nk-1)+1-n0) (fun i -> expr1 (n0+i) `cm.mult` expr2 (n0+i)));
+    //assert (subseq `equal` (init ((nk-1)+1-n0) (fun i -> expr1 (n0+i) `cm.mult` expr2 (n0+i))));
+    //assert (foldm_snoc cm (init ((nk-1)+1-n0) (fun i -> expr1 (n0+i) `cm.mult` expr2 (n0+i))) `eq.eq`
+    //       cm.mult (foldm_snoc cm (init ((nk-1)+1-n0) (fun i -> expr1 (n0+i)))) 
+    //               (foldm_snoc cm (init ((nk-1)+1-n0) (fun i -> expr2 (n0+i))))); 
+    //assert (foldm_snoc cm subseq `eq.eq` cm.mult (foldm_snoc cm (init ((nk-1)+1-n0) (fun i -> expr1 (n0+i)))) 
+    //               (foldm_snoc cm (init ((nk-1)+1-n0) (fun i -> expr2 (n0+i)))));  
+    let subfold_r1 = foldm_snoc cm subseq_r1 in
+    let subfold_r2 = foldm_snoc cm subseq_r2 in
+    lemma_eq_elim subseq_r1 (init ((nk-1)+1-n0) (fun i -> expr1 (n0+i)));
+    lemma_eq_elim subseq_r2 (init ((nk-1)+1-n0) (fun i -> expr2 (n0+i)));
+    //eq.reflexivity subfold_r1;
+    //eq.reflexivity subfold_r2; 
+    cm.congruence  (foldm_snoc cm (init ((nk-1)+1-n0) (fun i -> expr1 (n0+i)))) 
+                   (foldm_snoc cm (init ((nk-1)+1-n0) (fun i -> expr2 (n0+i))))
+                   subfold_r1
+                   subfold_r2;
+    let last_r1 = right_func1 (nk-n0) in
+    let last_r2 = right_func2 (nk-n0) in
+    //assert (subfold `eq.eq` cm.mult subfold_r1 subfold_r2);  
+    lemma_eq_elim (fst (un_snoc fullseq_r1)) subseq_r1; // subseq is literally (liat fullseq)
+    lemma_eq_elim (fst (un_snoc fullseq_r2)) subseq_r2; // subseq is literally (liat fullseq) 
+    //assert (last == last_r1 `cm.mult` last_r2);
+    //eq.reflexivity last;
+    //assert (lhs `eq.eq` (subfold `cm.mult` last));
+    //assert (lhs `eq.eq` (subfold `cm.mult` (last_r1 `cm.mult` last_r2)));
+    cm.congruence subfold last (subfold_r1 `cm.mult` subfold_r2) last;
+    //assert ((subfold `cm.mult` last) `eq.eq` ((subfold_r1 `cm.mult` subfold_r2) `cm.mult` last));
+    //eq.transitivity lhs (subfold `cm.mult` last) ((subfold_r1 `cm.mult` subfold_r2) `cm.mult` last);
+    //assert (lhs `eq.eq` ((subfold_r1 `cm.mult` subfold_r2) `cm.mult` (last_r1 `cm.mult` last_r2)));
+    aux_shuffle_lemma cm subfold_r1 subfold_r2 last_r1 last_r2;
+    //eq.transitivity lhs  
+    //                ((subfold_r1 `cm.mult` subfold_r2) `cm.mult` (last_r1 `cm.mult` last_r2))
+    //                ((subfold_r1 `cm.mult` last_r1) `cm.mult` (subfold_r2 `cm.mult` last_r2));
+    //assert (foldm_snoc cm fullseq_r1 == cm.mult last_r1 subfold_r1);
+    //cm.commutativity last_r1 subfold_r1;
+    //cm.commutativity last_r2 subfold_r2;
+    //eq.reflexivity (foldm_snoc cm fullseq_r1);  
+    //eq.reflexivity (foldm_snoc cm fullseq_r2);  
+    //eq.symmetry (cm.mult last_r1 subfold_r1) (cm.mult subfold_r1 last_r1);
+    //eq.symmetry (cm.mult last_r2 subfold_r2) (cm.mult subfold_r2 last_r2);
+    //assert (cm.mult subfold_r1 last_r1 `eq.eq` foldm_snoc cm fullseq_r1 ); 
+    //assert (cm.mult subfold_r2 last_r2 `eq.eq` foldm_snoc cm fullseq_r2 ); 
+    //assert (cm.mult last_r1 subfold_r1 == foldm_snoc cm fullseq_r1);
+    
+    cm.congruence (subfold_r1 `cm.mult` last_r1)
+                  (subfold_r2 `cm.mult` last_r2)
+                  (foldm_snoc cm fullseq_r1)
+                  (foldm_snoc cm fullseq_r2);
+    //eq.transitivity lhs
+    //                ((subfold_r1 `cm.mult` last_r1) `cm.mult` (subfold_r2 `cm.mult` last_r2))
+    //                ((foldm_snoc cm fullseq_r1) `cm.mult`  (foldm_snoc cm fullseq_r2));
+ 
+    ()
+) 
+
+
+
+let rec big_sum_exchange #c #eq (cm: Algebra.CommMonoid.Equiv.cm c eq) (m0: nat) (mk: nat{mk>=m0}) (n0: nat) (nk: nat{nk>=n0}) (expr: nat -> nat -> c) 
+  : Lemma (
+      big_sum cm m0 mk (fun (m:nat) -> big_sum cm n0 nk (fun (n:nat) -> expr m n)) `eq.eq` 
+      big_sum cm n0 nk (fun (n:nat) -> big_sum cm m0 mk (fun (m:nat) -> expr m n))           
+   ) = admit()
+
+
+//let poly_mul_nth_value #c (#r: commutative_ring #c) (p q: noncompact_poly_over_ring r) (deg: nat{deg < length p * length q})
+//  : Lemma (nth (poly_mul p q) deg == 
 
 let poly_mul_is_commutative #c (#r: commutative_ring #c) (p q: noncompact_poly_over_ring r) 
   : Lemma (ensures poly_mul p q `noncompact_poly_eq` poly_mul q p) =  
@@ -218,7 +666,18 @@ let poly_mul_is_associative #c (#r: commutative_ring #c) (p q w: noncompact_poly
   : Lemma (ensures poly_mul p (poly_mul q w) `ncpoly_eq` poly_mul (poly_mul p q) w) = admit()
 
 let poly_mul_left_distributivity #c (#r: commutative_ring #c) (p q w: noncompact_poly_over_ring r)
-  : Lemma (poly_mul p (noncompact_poly_add q w) `ncpoly_eq` noncompact_poly_add (poly_mul p q) (poly_mul p w)) = admit()
+  : Lemma (poly_mul p (noncompact_poly_add q w) `ncpoly_eq` noncompact_poly_add (poly_mul p q) (poly_mul p w)) = 
+  if is_empty p || is_empty q || is_empty w then admit() else (
+  let lhs = poly_product_monomial_matrix p (noncompact_poly_add q w) in
+  let cm = poly_add_commutative_monoid r in
+  let rhs = noncompact_poly_add
+    (Seq.Permutation.foldm_snoc cm (poly_product_monomial_matrix p q))
+    (Seq.Permutation.foldm_snoc cm (poly_product_monomial_matrix p w)) in
+  Seq.Permutation.
+  
+  admit();
+  ()
+  )
   
 let poly_mul_right_distributivity #c (#r: commutative_ring #c) (p q w: noncompact_poly_over_ring r)
   : Lemma (poly_mul (noncompact_poly_add p q) w `ncpoly_eq` noncompact_poly_add (poly_mul p w) (poly_mul q w)) = admit()
